theories/stacked_borrows/primitive_laws.v
@@ -1,42 +1,5 @@
-(** This file proves the basic laws of the BorIngLang program logic by applying
-the Simuliris lifting lemmas. *)
-
+(* Re-export steps *)
 From iris.proofmode Require Export tactics.
-From iris.bi.lib Require Import fractional.
-From iris.base_logic.lib Require Import ghost_map.
 From simuliris.base_logic Require Export gen_sim_heap gen_sim_prog.
 From simuliris.simulation Require Export slsls.
-From simuliris.simulation Require Import lifting.
-From simuliris.stacked_borrows Require Export class_instances tactics notation heap steps_refl steps_opt.
-From iris.prelude Require Import options.
-
-
-
-(** Program assertions *)
-Notation "f '@t' Kt" := (hasfun (hG:=gen_prog_inG_target) f Kt)
-  (at level 20, format "f  @t  Kt") : bi_scope.
-Notation "f '@s' Ks" := (hasfun (hG:=gen_prog_inG_source) f Ks)
-  (at level 20, format "f  @s  Ks") : bi_scope.
-
-
-Section lifting.
-Context `{!sborG Σ}.
-Implicit Types P Q : iProp Σ.
-Implicit Types Φ : result → result → iProp Σ.
-Implicit Types σ σ_s σ_t : state.
-Implicit Types r r_s r_t : result.
-Implicit Types l : loc.
-Implicit Types f : fname.
-
-Context (Ω : result → result → iProp Σ).
-
-
-(** Program for target *)
-Lemma hasfun_target_agree f K_t1 K_t2 : f @t K_t1 -∗ f @t K_t2 -∗ ⌜K_t1 = K_t2⌝.
-Proof. apply hasfun_agree. Qed.
-
-(** Program for source *)
-Lemma hasfun_source_agree f K_s1 K_s2 : f @s K_s1 -∗ f @s K_s2 -∗ ⌜K_s1 = K_s2⌝.
-Proof. apply hasfun_agree. Qed.
-
-End lifting.
+From simuliris.stacked_borrows Require Export class_instances tactics notation defs logical_state steps_refl steps_opt.
